\documentclass{article}
\usepackage{amsmath}

\begin{document}

\begin{align*}
A(n) &= A(n-1) + 2C(n-1) + E(n-1) + I(n-1), \quad &A(2) &= 1 \\
B(n) &= 2E(n-1), \quad &B(2) &= 0 \\
C(n) &= E(n-1), \quad &C(2) &= 0 \\
D(n) &= 2A(n-1) + C(n-1) + E(n-1) + F(n-1) + G(n-1) + H(n-1), \quad &D(2) &= 1 \\
E(n) &= 2C(n-1), \quad &E(2) &= 1 \\
F(n) &= 2A(n-1) + 2B(n-1) + 2C(n-1) + 2D(n-1) + 2G(n-1), \quad &F(2) &= 2 \\
G(n) &= A(n-1) + C(n-1) + G(n-1), \quad &G(2) &= 1 \\
H(n) &= E(n-1) + H(n-1), \quad &H(2) &= 0 \\
I(n) &= A(n-1) + C(n-1) + E(n-1) + G(n-1) + H(n-1), \quad &I(2) &= 1 \\
\text{counts}(n) &= 2A(n) + 2C(n) + 2E(n) + F(n) + 2I(n)
\end{align*}

\end{document}
