\documentclass{article}
\usepackage{amsmath}

\begin{document}

\scriptsize
\begin{align*}
A(n) &= 3 + 2A(n-1) + B(n-1) + 3C(n-1) + 2E(n-1) + I(n-1), &A(1) &= 0 \\
B(n) &= 3 + 2A(n-1) + B(n-1) + 2C(n-1) + 2E(n-1), &B(1) &= 0 \\
C(n) &= 1 + C(n-1) + E(n-1), &C(1) &= 0 \\
D(n) &= 2 + 3A(n-1) + B(n-1) + C(n-1) + D(n-1) + E(n-1) + F(n-1) + G(n-1) + H(n-1), &D(1) &= 0 \\
E(n) &= 1 + 2C(n-1) + E(n-1), &E(1) &= 0 \\
F(n) &= 3 + 4A(n-1) + 2B(n-1) + 2C(n-1) + 2D(n-1) + F(n-1) + 2G(n-1), &F(1) &= 0 \\
G(n) &= 1 + A(n-1) + C(n-1) + G(n-1), &G(1) &= 0 \\
H(n) &= E(n-1) + H(n-1), &H(1) &= 0 \\
I(n) &= 1 + A(n-1) + C(n-1) + E(n-1) + G(n-1) + H(n-1), &I(1) &= 0 \\
\text{counts}(n) &= \text{counts}(n-1) + 3 + 6A(n) + 3B(n) + 4C(n) + 2D(n) + 3E(n) + F(n) + 2I(n), &\text{counts}(1) &= 1
\end{align*}

\end{document}
